src/Curve25519_Hop1.ec
@@ -1,15 +1,15 @@
 require import Bool List Int IntDiv CoreMap Real Ring StdOrder Zp_25519.
 require import Curve25519_Spec.
-import Zp_25519 ZModpRing Ring.IntID.
+import Zp_25519  Ring.IntID Zp_25519.ZModpRing.
 
 from Jasmin require import JModel.
 
 (* exp exp *)
 lemma expE (z : zp) (e1 e2 : int) : 0 <= e1 /\ 0 <= e2 =>
-  ZModpRing.exp (ZModpRing.exp z e1) e2 =
-  ZModpRing.exp z (e1*e2).
+    ZModpRing.exp (ZModpRing.exp z e1) e2 =
+    ZModpRing.exp z (e1*e2).
 proof.
- rewrite -ZModpRing.exprM => />.
+    rewrite -ZModpRing.exprM => />.
 qed.
 
 (* returns the first 2 elements of the input triple *)
@@ -19,16 +19,16 @@ op select_tuple_12 (t : ('a * 'a) * ('a * 'a) * 'c) = (t.`1, t.`2).
   (*  - this op returns the first 2 elements in
   the correct order       *)
 op reconstruct_tuple (t : ('a * 'a) * ('a * 'a) * bool) =
-  if t.`3
-  then swap_tuple (select_tuple_12 t)
-  else select_tuple_12 t.
+    if t.`3
+    then swap_tuple (select_tuple_12 t)
+    else select_tuple_12 t.
 
 lemma eq_reconstruct_select_tuple (t : (('a * 'a) * ('a * 'a) * bool)) :
-  t.`3 = false => 
-  select_tuple_12 t = reconstruct_tuple t.
+    t.`3 = false => 
+    select_tuple_12 t = reconstruct_tuple t.
 proof.
-  rewrite /reconstruct_tuple /select_tuple_12.
-  by move => ? /#.
+    rewrite /reconstruct_tuple /select_tuple_12.
+    by move => ? /#.
 qed.
 
 (* similar to foldl_in_eq -- the proof is basically the same -- defined in JMemory *)
@@ -39,15 +39,16 @@ lemma foldl_in_eq_r (f1 : 'a1 -> 'b -> 'a1)
                     (s  : 'b list)
                     (a2 : 'a2)
                     (r  : 'a2 -> 'a1) :
-(forall a2 b, b \in s => f1 (r a2) b = r (f2 a2 b)) => foldl f1 (r a2) s = r (foldl f2 a2 s).
+    (forall a2 b, b \in s => f1 (r a2) b = r (f2 a2 b)) => 
+                        foldl f1 (r a2) s = r (foldl f2 a2 s).
 proof.
-  move: s a2. elim.
-  by move => a2.
-  move => x l hrec a2 /= hin. rewrite hin.
-  by left.
-  rewrite hrec //; move => ? ? h; rewrite hin.
-  by right.
-  by trivial.
+    move: s a2. elim.
+        by move => a2.
+    move => x l hrec a2 /= hin. rewrite hin.
+    by left.
+    rewrite hrec //; move => ? ? h; rewrite hin.
+        by right.
+    by trivial.
 qed.
 
 (** step1: add_and_double = add_and_double1 : reordered to match implementation **)
@@ -76,357 +77,354 @@ op add_and_double1 (qx : zp) (nqs : (zp * zp) * (zp * zp)) =
   in  ((x2,z2), (x3,z3)).
 
 lemma eq_add_and_double1 (qx : zp) (nqs : (zp * zp) * (zp * zp)) :
-  add_and_double qx nqs = add_and_double1 qx nqs.
+    add_and_double qx nqs = add_and_double1 qx nqs.
 proof.
-  rewrite /add_and_double /add_and_double1.
-  simplify => /#.
+    rewrite /add_and_double /add_and_double1.
+    simplify => /#.
 qed.
 
 op montgomery_ladder1(init : zp, k : W256.t) =
-  let nqs0 = ((Zp_25519.one,Zp_25519.zero),(init,Zp_25519.one)) in
-  foldl (fun (nqs : (zp * zp) * (zp * zp)) ctr => 
+    let nqs0 = ((Zp_25519.one,Zp_25519.zero),(init,Zp_25519.one)) in
+    foldl (fun (nqs : (zp * zp) * (zp * zp)) ctr => 
          if ith_bit k ctr
          then swap_tuple (add_and_double1 init (swap_tuple(nqs)))
          else add_and_double1 init nqs) nqs0 (rev (iota_ 0 255)).
 
 (* lemma: montgomery_ladder = montgomery_ladder1 *)
 lemma eq_montgomery_ladder1 (init : zp) (k : W256.t) :
-  montgomery_ladder init k = montgomery_ladder1 init k.
+    montgomery_ladder init k = montgomery_ladder1 init k.
 proof.
-  rewrite /montgomery_ladder /montgomery_ladder1 /=.
-  apply foldl_in_eq.
-  move => nqs ctr inlist => /=.
-  case (ith_bit k ctr).
-    by move => ?; rewrite /swap_tuple /#.
+    rewrite /montgomery_ladder /montgomery_ladder1 /=.
+    apply foldl_in_eq.
+    move => nqs ctr inlist => /=.
+    case (ith_bit k ctr).
+        by move => ?; rewrite /swap_tuple /#.
     by move => ?; rewrite /swap_tuple /#.
 qed.
 
 (** step 2: isolate foldl function and introduce reconstruct tuple **)
 op montgomery_ladder2_step(k : W256.t, init : zp, nqs : (zp * zp) * (zp * zp), ctr : int) =
-  if ith_bit k ctr
-  then swap_tuple(add_and_double1 init (swap_tuple(nqs)))
-  else add_and_double1 init nqs.
+    if ith_bit k ctr
+    then swap_tuple(add_and_double1 init (swap_tuple(nqs)))
+    else add_and_double1 init nqs.
 
 op montgomery_ladder2(init : zp, k : W256.t) =
-  let nqs0 = reconstruct_tuple ((Zp_25519.one,Zp_25519.zero),(init,Zp_25519.one),false) in
-  foldl (montgomery_ladder2_step k init) nqs0 (rev (iota_ 0 255)).
+    let nqs0 = reconstruct_tuple ((Zp_25519.one,Zp_25519.zero),(init,Zp_25519.one),false) in
+    foldl (montgomery_ladder2_step k init) nqs0 (rev (iota_ 0 255)).
 
 (* lemma: montgomery_ladder1 = montgomery_ladder2 *)
 lemma eq_montgomery_ladder2 (init : zp) (k : W256.t) :
-  montgomery_ladder1 init k = montgomery_ladder2 init k.
+    montgomery_ladder1 init k = montgomery_ladder2 init k.
 proof.
-  rewrite /montgomery_ladder1 /montgomery_ladder2 /reconstruct_tuple /select_tuple_12.
-  rewrite /montgomery_ladder2_step.
-  by simplify.
+    rewrite /montgomery_ladder1 /montgomery_ladder2 /reconstruct_tuple /select_tuple_12.
+    rewrite /montgomery_ladder2_step.
+    by simplify.
 qed.
 
 (** step 3: extend the state to contain an additional bit stating if the state is swapped **)
 op cswap( t : ('a * 'a) * ('a * 'a), b : bool ) = 
-  if b
-  then swap_tuple t
-  else t.
+    if b
+    then swap_tuple t
+    else t.
 
 op montgomery_ladder3_step(k : W256.t, init : zp, nqs : (zp * zp) * (zp * zp) * bool, ctr : int) =
-  let nqs = cswap (select_tuple_12 nqs) (nqs.`3 ^^ (ith_bit k ctr)) in
-  let nqs = add_and_double1 init nqs in
-  (nqs.`1, nqs.`2, (ith_bit k ctr)).
+    let nqs = cswap (select_tuple_12 nqs) (nqs.`3 ^^ (ith_bit k ctr)) in
+    let nqs = add_and_double1 init nqs in
+    (nqs.`1, nqs.`2, (ith_bit k ctr)).
 
 op montgomery_ladder3(init : zp, k : W256.t) =
-  let nqs0 = ((Zp_25519.one,Zp_25519.zero),(init,Zp_25519.one),false) in
-  foldl (montgomery_ladder3_step k init) nqs0 (rev (iota_ 0 255)).
+    let nqs0 = ((Zp_25519.one,Zp_25519.zero),(init,Zp_25519.one),false) in
+    foldl (montgomery_ladder3_step k init) nqs0 (rev (iota_ 0 255)).
 
 lemma eq_montgomery_ladder3_reconstruct (init : zp) (k: W256.t) :
-  montgomery_ladder2 init k = reconstruct_tuple (montgomery_ladder3 init k).
+    montgomery_ladder2 init k = reconstruct_tuple (montgomery_ladder3 init k).
 proof.
-  rewrite /montgomery_ladder2 /montgomery_ladder3 //=.
-  apply foldl_in_eq_r.
-  move => ? ? ?.
-  rewrite /reconstruct_tuple /montgomery_ladder2_step /montgomery_ladder3_step.
-  rewrite /swap_tuple /select_tuple_12 /cswap.
-  simplify => /#.
+    rewrite /montgomery_ladder2 /montgomery_ladder3 //=.
+    apply foldl_in_eq_r.
+    move => ? ? ?.
+    rewrite /reconstruct_tuple /montgomery_ladder2_step /montgomery_ladder3_step.
+    rewrite /swap_tuple /select_tuple_12 /cswap.
+    simplify => /#.
 qed.
     
 (* lemma: if the first bit of k is 0, which will be because of decodeScalar25519, *)
 (*  then montgomery_ladder2 = select_tuple_12 montgomery_ladder3 *)
 lemma eq_montgomery_ladder3 (init : zp) (k: W256.t) :
-  k.[0] = false =>
-  montgomery_ladder2 init k = select_tuple_12 (montgomery_ladder3 init k).
+    k.[0] = false =>
+    montgomery_ladder2 init k = select_tuple_12 (montgomery_ladder3 init k).
 proof.
-  move => hkf.  
-  have tbf : (montgomery_ladder3 init k).`3 = false. (*third bit false*)
-  rewrite /montgomery_ladder3 /montgomery_ladder3_step /select_tuple_12 /cswap /ith_bit /swap_tuple => />.
-  rewrite foldl_rev; auto => />; rewrite -iotaredE => />.  
-  
-  have seqr : select_tuple_12 (montgomery_ladder3 init k) = (*select eq reconstruct*)
-              reconstruct_tuple (montgomery_ladder3 init k).
-    by apply /eq_reconstruct_select_tuple /tbf.
-  rewrite seqr.
+    move => hkf.  
+    have tbf : (montgomery_ladder3 init k).`3 = false. (*third bit false*)
+    rewrite /montgomery_ladder3 /montgomery_ladder3_step /select_tuple_12 /cswap /ith_bit /swap_tuple => />.
+    rewrite foldl_rev; auto => />; rewrite -iotaredE => />.  
+    have seqr : select_tuple_12 (montgomery_ladder3 init k) = reconstruct_tuple (montgomery_ladder3 init k).
+        by apply /eq_reconstruct_select_tuple /tbf.
+    rewrite seqr.
     by apply eq_montgomery_ladder3_reconstruct.
 qed.
 
 (** step 4: montgomery_ladder = select_tuple_12 montgomery_ladder3 **)
 lemma eq_montgomery_ladder123 (init : zp) (k: W256.t) :
-  k.[0] = false => montgomery_ladder init k = select_tuple_12 (montgomery_ladder3 init k).
+    k.[0] = false => montgomery_ladder init k = select_tuple_12 (montgomery_ladder3 init k).
 proof.
-  move => H.
-  rewrite eq_montgomery_ladder1 eq_montgomery_ladder2 eq_montgomery_ladder3. apply H.
-  trivial.
+    move => H.
+    rewrite eq_montgomery_ladder1 eq_montgomery_ladder2 eq_montgomery_ladder3. apply H.
+    trivial.
 qed.
 
 (** step 5: introduce reordering in encode point **)
 (*  - we split invert in 3 parts to make the proof faster *)
 op invert_p_p1(z1 : zp) : (zp*zp) =
-  let z2 = exp z1 2 in
-  let z8 = exp z2 (2*2) in
-  let z9 = Zp_25519.( * ) z1 z8 in
-  let z11 = Zp_25519.( * ) z2 z9 in
-  let z22 = exp z11 2 in
-  let z_5_0 = Zp_25519.( * ) z9 z22 in
-  (z_5_0, z11).
+    let z2 = exp z1 2 in
+    let z8 = exp z2 (2*2) in
+    let z9 = Zp_25519.( * ) z1 z8 in
+    let z11 = Zp_25519.( * ) z2 z9 in
+    let z22 = exp z11 2 in
+    let z_5_0 = Zp_25519.( * ) z9 z22 in
+        (z_5_0, z11).
 
 op invert_p_p2(z_5_0 : zp) : zp = 
-  let z_10_5 = ZModpRing.exp z_5_0 (2^5) in
-  let z_10_0 = Zp_25519.( * ) z_10_5 z_5_0 in
-  let z_20_10 = ZModpRing.exp z_10_0 (2^10) in
-  let z_20_0 = Zp_25519.( * ) z_20_10 z_10_0 in
-  let z_40_20 = ZModpRing.exp z_20_0 (2^20) in
-  let z_40_0 = Zp_25519.( * ) z_40_20 z_20_0 in
-  let z_50_10 = ZModpRing.exp z_40_0 (2^10) in
-  let z_50_0 = Zp_25519.( * ) z_50_10 z_10_0 in
-  z_50_0.
+    let z_10_5 = ZModpRing.exp z_5_0 (2^5) in
+    let z_10_0 = Zp_25519.( * ) z_10_5 z_5_0 in
+    let z_20_10 = ZModpRing.exp z_10_0 (2^10) in
+    let z_20_0 = Zp_25519.( * ) z_20_10 z_10_0 in
+    let z_40_20 = ZModpRing.exp z_20_0 (2^20) in
+    let z_40_0 = Zp_25519.( * ) z_40_20 z_20_0 in
+    let z_50_10 = ZModpRing.exp z_40_0 (2^10) in
+    let z_50_0 = Zp_25519.( * ) z_50_10 z_10_0 in
+        z_50_0.
 
 op invert_p_p3(z_50_0 z11 : zp) : zp =
-  let z_100_50 = ZModpRing.exp z_50_0 (2^50) in
-  let z_100_0 = Zp_25519.( * ) z_100_50 z_50_0 in
-  let z_200_100 = ZModpRing.exp z_100_0 (2^100) in
-  let z_200_0 = Zp_25519.( * ) z_200_100 z_100_0 in
-  let z_250_50 = ZModpRing.exp z_200_0 (2^50) in
-  let z_250_0 = Zp_25519.( * ) z_250_50 z_50_0 in
-  let z_255_5 = ZModpRing.exp z_250_0 (2^5) in
-  let z_255_21 = Zp_25519.( * ) z_255_5 z11 in
-  z_255_21.
+    let z_100_50 = ZModpRing.exp z_50_0 (2^50) in
+    let z_100_0 = Zp_25519.( * ) z_100_50 z_50_0 in
+    let z_200_100 = ZModpRing.exp z_100_0 (2^100) in
+    let z_200_0 = Zp_25519.( * ) z_200_100 z_100_0 in
+    let z_250_50 = ZModpRing.exp z_200_0 (2^50) in
+    let z_250_0 = Zp_25519.( * ) z_250_50 z_50_0 in
+    let z_255_5 = ZModpRing.exp z_250_0 (2^5) in
+    let z_255_21 = Zp_25519.( * ) z_255_5 z11 in
+        z_255_21    .
 
 op invert_p(z1 : zp) : zp =
-  let (z_5_0, z11) = invert_p_p1 z1 in
-  let z_50_0 = invert_p_p2 z_5_0 in
-  let z_255_21 = invert_p_p3 z_50_0 z11 in
-  z_255_21 axiomatized by invert_pE.
+    let (z_5_0, z11) = invert_p_p1 z1 in
+    let z_50_0 = invert_p_p2 z_5_0 in
+    let z_255_21 = invert_p_p3 z_50_0 z11 in
+    z_255_21 axiomatized by invert_pE.
 
 lemma eq_invert_p (z1: zp) :
-  invert_p z1 = ZModpRing.exp z1 (p-2).
+    invert_p z1 = ZModpRing.exp z1 (p-2).
 proof.
-rewrite invert_pE.
-(*invert_p1*)
-  rewrite /invert_p_p1 /= expE //= /invert_p_p3 /invert_p_p2 //=. 
-  rewrite -!exprS // -!exprD_nneg => />. rewrite -!exprM -!exprD_nneg => />.
-  rewrite -!exprM => />. rewrite -!exprD_nneg => />. rewrite -!exprM => />.
-  rewrite -!exprD_nneg => />. rewrite -!exprM => />. rewrite -!exprD_nneg => />.
-  rewrite -!exprM => />. rewrite -!exprD_nneg => />. rewrite -!exprM => />.
-  rewrite -!exprD_nneg => />. rewrite -!exprM => />. rewrite -!exprD_nneg => />.
-  rewrite -!exprM => />. rewrite -exprD_nneg => />. rewrite -exprM => />.
-  rewrite -!exprD_nneg => />. rewrite pE => />.
+    rewrite invert_pE.
+    rewrite /invert_p_p1 /= expE //= /invert_p_p3 /invert_p_p2 //=. 
+    rewrite -!exprS // -!exprD_nneg => />. rewrite -!exprM -!exprD_nneg => />.
+    rewrite -!exprM => />. rewrite -!exprD_nneg => />. rewrite -!exprM => />.
+    rewrite -!exprD_nneg => />. rewrite -!exprM => />. rewrite -!exprD_nneg => />.
+    rewrite -!exprM => />. rewrite -!exprD_nneg => />. rewrite -!exprM => />.
+    rewrite -!exprD_nneg => />. rewrite -!exprM => />. rewrite -!exprD_nneg => />.
+    rewrite -!exprM => />. rewrite -exprD_nneg => />. rewrite -exprM => />.
+    rewrite -!exprD_nneg => />. rewrite pE => />.
 qed. (* there must be a faster and elegant way of doing this *)
 
 (* now we define invert as one op and prove it equiv to exp z1 (p-2) *)
 op invert0(z1 : zp) : zp =
-  let z2 = ZModpRing.exp z1 2 in
-  let z8 = ZModpRing.exp z2 (2*2) in
-  let z9 = Zp_25519.( * ) z1 z8 in
-  let z11 = Zp_25519.( * ) z2 z9 in
-  let z22 = ZModpRing.exp z11 2 in
-  let z_5_0 =  Zp_25519.( * ) z9 z22 in
-  let z_10_5 = ZModpRing.exp z_5_0 (2^5) in
-  let z_10_0 =  Zp_25519.( * ) z_10_5 z_5_0 in
-  let z_20_10 = ZModpRing.exp z_10_0 (2^10) in
-  let z_20_0 =  Zp_25519.( * ) z_20_10 z_10_0 in
-  let z_40_20 = ZModpRing.exp z_20_0 (2^20) in
-  let z_40_0 =  Zp_25519.( * ) z_40_20 z_20_0 in
-  let z_50_10 = ZModpRing.exp z_40_0 (2^10) in
-  let z_50_0 =  Zp_25519.( * ) z_50_10 z_10_0 in
-  let z_100_50 = ZModpRing.exp z_50_0 (2^50) in
-  let z_100_0 =  Zp_25519.( * ) z_100_50 z_50_0 in
-  let z_200_100 = ZModpRing.exp z_100_0 (2^100) in
-  let z_200_0 =  Zp_25519.( * ) z_200_100 z_100_0 in
-  let z_250_50 = ZModpRing.exp z_200_0 (2^50) in
-  let z_250_0 =  Zp_25519.( * ) z_250_50 z_50_0 in
-  let z_255_5 = ZModpRing.exp z_250_0 (2^5) in
-  let z_255_21 =  Zp_25519.( * ) z_255_5 z11 in
-  z_255_21 axiomatized by invert0E.
+    let z2 = ZModpRing.exp z1 2 in
+    let z8 = ZModpRing.exp z2 (2*2) in
+    let z9 = Zp_25519.( * ) z1 z8 in
+    let z11 = Zp_25519.( * ) z2 z9 in
+    let z22 = ZModpRing.exp z11 2 in
+    let z_5_0 =  Zp_25519.( * ) z9 z22 in
+    let z_10_5 = ZModpRing.exp z_5_0 (2^5) in
+    let z_10_0 =  Zp_25519.( * ) z_10_5 z_5_0 in
+    let z_20_10 = ZModpRing.exp z_10_0 (2^10) in
+    let z_20_0 =  Zp_25519.( * ) z_20_10 z_10_0 in
+    let z_40_20 = ZModpRing.exp z_20_0 (2^20) in
+    let z_40_0 =  Zp_25519.( * ) z_40_20 z_20_0 in
+    let z_50_10 = ZModpRing.exp z_40_0 (2^10) in
+    let z_50_0 =  Zp_25519.( * ) z_50_10 z_10_0 in
+    let z_100_50 = ZModpRing.exp z_50_0 (2^50) in
+    let z_100_0 =  Zp_25519.( * ) z_100_50 z_50_0 in
+    let z_200_100 = ZModpRing.exp z_100_0 (2^100) in
+    let z_200_0 =  Zp_25519.( * ) z_200_100 z_100_0 in
+    let z_250_50 = ZModpRing.exp z_200_0 (2^50) in
+    let z_250_0 =  Zp_25519.( * ) z_250_50 z_50_0 in
+    let z_255_5 = ZModpRing.exp z_250_0 (2^5) in
+    let z_255_21 =  Zp_25519.( * ) z_255_5 z11 in
+        z_255_21 axiomatized by invert0E.
 
 lemma eq_invert0 (z1 : zp) :
-  invert0 z1 = invert_p z1.
+    invert0 z1 = invert_p z1.
 proof.
-  rewrite invert0E invert_pE /invert_p_p1 /invert_p_p2 /invert_p_p3 //.
+    rewrite invert0E invert_pE /invert_p_p1 /invert_p_p2 /invert_p_p3 //.
 qed.
 
 lemma eq_invert0p (z1 : zp) :
-  invert0 z1 = ZModpRing.exp z1 (p-2).
+    invert0 z1 = ZModpRing.exp z1 (p-2).
 proof.
-  rewrite eq_invert0 eq_invert_p //.
+    rewrite eq_invert0 eq_invert_p //.
 qed.
 
 op sqr(z : zp) : zp =
- ZModpRing.exp z 2.
+    ZModpRing.exp z 2.
 
 op it_sqr(e : int, z : zp) : zp =
-  ZModpRing.exp z (2^e).
+    ZModpRing.exp z (2^e).
 
 op it_sqr1(e : int, z : zp) : zp =
-  foldl (fun (z' : zp) _ => exp z' 2) z (iota_ 0 e).
+    foldl (fun (z' : zp) _ => exp z' 2) z (iota_ 0 e).
 
 lemma eq_it_sqr1 (e : int, z : zp) :
-  0 <= e  =>
-  it_sqr1 e z = it_sqr e z.
+    0 <= e  =>
+    it_sqr1 e z = it_sqr e z.
 proof.
-  move : e.
-  rewrite /it_sqr1 /it_sqr. elim. simplify. rewrite -iotaredE expr1 //. 
-  move => i ige0 hin.
-  rewrite iotaSr // -cats1 foldl_cat hin /= expE /=.  smt(gt0_pow2).
-  congr. clear hin.
-  rewrite exprS // mulzC //.
+    move : e.
+    rewrite /it_sqr1 /it_sqr. elim. simplify. rewrite -iotaredE expr1 //. 
+    move => i ige0 hin.
+    rewrite iotaSr // -cats1 foldl_cat hin /= expE /=.  smt(gt0_pow2).
+    congr. clear hin.
+    rewrite exprS // mulzC //.
 qed.
 
 op invert1(z1 : zp) : zp =
-  let t0 = sqr z1  in        (* z1^2  *)
-  let t1 = sqr t0  in        (* z1^4  *)
-  let t1 = sqr t1  in        (* z1^8  *)
-  let t1 =  Zp_25519.( * ) z1 t1 in        (* z1^9  *)
-  let t0 =  Zp_25519.( * ) t0 t1 in        (* z1^11 *)
-  let t2 = sqr t0  in        (* z1^22 *)
-  let t1 =  Zp_25519.( * ) t1 t2 in        (* z_5_0  *)
-  let t2 = sqr t1  in        (* z_10_5 *) 
-  let t2 = it_sqr 4 t2  in
-  let t1 =  Zp_25519.( * ) t1 t2 in        (* z_10_0 *)
-  let t2 = it_sqr 10 t1 in   (* z_20_10 *)
-  let t2 =  Zp_25519.( * ) t1 t2 in        (* z_20_0 *)
-  let t3 = it_sqr 20 t2 in   (* z_40_20 *)
-  let t2 =  Zp_25519.( * ) t2 t3 in        (* z_40_0 *)
-  let t2 = it_sqr 10 t2 in   (* z_50_10 *)
-  let t1 =  Zp_25519.( * ) t1 t2 in        (* z_50_0 *)
-  let t2 = it_sqr 50 t1 in   (* z_100_50 *)
-  let t2 =  Zp_25519.( * ) t1 t2 in        (* z_100_0 *)
-  let t3 = it_sqr 100 t2 in  (* z_200_100 *)
-  let t2 =  Zp_25519.( * ) t2 t3 in        (* z_200_0 *)
-  let t2 = it_sqr 50 t2 in   (* z_250_50 *)
-  let t1 =  Zp_25519.( * ) t1 t2 in        (* z_250_0 *)
-  let t1 = it_sqr 4 t1 in    (* z_255_5 *) 
-  let t1 = sqr t1 in
-  let t1 =  Zp_25519.( * ) t0 t1 in
-  t1 axiomatized by invert1E.
+    let t0 = sqr z1  in        (* z1^2  *)
+    let t1 = sqr t0  in        (* z1^4  *)
+    let t1 = sqr t1  in        (* z1^8  *)
+    let t1 = Zp_25519.( * ) z1 t1 in        (* z1^9  *)
+    let t0 = Zp_25519.( * ) t0 t1 in        (* z1^11 *)
+    let t2 = sqr t0  in        (* z1^22 *)
+    let t1 = Zp_25519.( * ) t1 t2 in        (* z_5_0  *)
+    let t2 = sqr t1  in        (* z_10_5 *) 
+    let t2 = it_sqr 4 t2  in
+    let t1 = Zp_25519.( * ) t1 t2 in        (* z_10_0 *)
+    let t2 = it_sqr 10 t1 in   (* z_20_10 *)
+    let t2 = Zp_25519.( * ) t1 t2 in        (* z_20_0 *)
+    let t3 = it_sqr 20 t2 in   (* z_40_20 *)
+    let t2 = Zp_25519.( * ) t2 t3 in        (* z_40_0 *)
+    let t2 = it_sqr 10 t2 in   (* z_50_10 *)
+    let t1 = Zp_25519.( * ) t1 t2 in        (* z_50_0 *)
+    let t2 = it_sqr 50 t1 in   (* z_100_50 *)
+    let t2 = Zp_25519.( * ) t1 t2 in        (* z_100_0 *)
+    let t3 = it_sqr 100 t2 in  (* z_200_100 *)
+    let t2 = Zp_25519.( * ) t2 t3 in        (* z_200_0 *)
+    let t2 = it_sqr 50 t2 in   (* z_250_50 *)
+    let t1 = Zp_25519.( * ) t1 t2 in        (* z_250_0 *)
+    let t1 = it_sqr 4 t1 in    (* z_255_5 *) 
+    let t1 = sqr t1 in
+    let t1 = Zp_25519.( * ) t0 t1 in
+        t1 axiomatized by invert1E.
 
 lemma eq_invert1 (z1: zp) :
-  invert1 z1 = invert0 z1.
+    invert1 z1 = invert0 z1.
 proof.
- rewrite invert1E invert0E /= /it_sqr /sqr /=.
- smt(exprS exprD expE).
+    rewrite invert1E invert0E /= /it_sqr /sqr /=.
+    smt(exprS exprD expE).
 qed.
 
 (** split invert2 in 3 parts : jump from it_sqr to it_sqr1 **)
 
 op invert2(z1 : zp) : zp =
-  let t0 = sqr z1  in        (* z1^2  *)
-  let t1 = sqr t0  in        (* z1^4  *)
-  let t1 = sqr t1  in        (* z1^8  *)
-  let t1 =  Zp_25519.( * ) z1 t1 in        (* z1^9  *)
-  let t0 =  Zp_25519.( * ) t0 t1 in        (* z1^11 *)
-  let t2 = sqr t0  in        (* z1^22 *)
-  let t1 =  Zp_25519.( * ) t1 t2 in        (* z_5_0  *)
-  let t2 = sqr t1  in        (* z_10_5 *) 
-  let t2 = it_sqr1 4 t2  in
-  let t1 =  Zp_25519.( * ) t1 t2 in        (* z_10_0 *)
-  let t2 = it_sqr1 10 t1 in  (* z_20_10 *)
-  let t2 =  Zp_25519.( * ) t1 t2 in        (* z_20_0 *)
-  let t3 = it_sqr1 20 t2 in  (* z_40_20 *)
-  let t2 =  Zp_25519.( * ) t2 t3 in        (* z_40_0 *)
-  let t2 = it_sqr1 10 t2 in  (* z_50_10 *)
-  let t1 =  Zp_25519.( * ) t1 t2 in        (* z_50_0 *)
-  let t2 = it_sqr1 50 t1 in  (* z_100_50 *)
-  let t2 =  Zp_25519.( * ) t1 t2 in        (* z_100_0 *)
-  let t3 = it_sqr1 100 t2 in (* z_200_100 *)
-  let t2 =  Zp_25519.( * ) t2 t3 in        (* z_200_0 *)
-  let t2 = it_sqr1 50 t2 in  (* z_250_50 *)
-  let t1 =  Zp_25519.( * ) t1 t2 in        (* z_250_0 *)
-  let t1 = it_sqr1 4 t1 in   (* z_255_5 *) 
-  let t1 = sqr t1 in
-  let t1 =  Zp_25519.( * ) t0 t1 in
-  t1 axiomatized by invert2E.
+    let t0 = sqr z1  in        (* z1^2  *)
+    let t1 = sqr t0  in        (* z1^4  *)
+    let t1 = sqr t1  in        (* z1^8  *)
+    let t1 =  Zp_25519.( * ) z1 t1 in        (* z1^9  *)
+    let t0 =  Zp_25519.( * ) t0 t1 in        (* z1^11 *)
+    let t2 = sqr t0  in        (* z1^22 *)
+    let t1 =  Zp_25519.( * ) t1 t2 in        (* z_5_0  *)
+    let t2 = sqr t1  in        (* z_10_5 *) 
+    let t2 = it_sqr1 4 t2  in
+    let t1 =  Zp_25519.( * ) t1 t2 in        (* z_10_0 *)
+    let t2 = it_sqr1 10 t1 in  (* z_20_10 *)
+    let t2 =  Zp_25519.( * ) t1 t2 in        (* z_20_0 *)
+    let t3 = it_sqr1 20 t2 in  (* z_40_20 *)
+    let t2 =  Zp_25519.( * ) t2 t3 in        (* z_40_0 *)
+    let t2 = it_sqr1 10 t2 in  (* z_50_10 *)
+    let t1 =  Zp_25519.( * ) t1 t2 in        (* z_50_0 *)
+    let t2 = it_sqr1 50 t1 in  (* z_100_50 *)
+    let t2 =  Zp_25519.( * ) t1 t2 in        (* z_100_0 *)
+    let t3 = it_sqr1 100 t2 in (* z_200_100 *)
+    let t2 =  Zp_25519.( * ) t2 t3 in        (* z_200_0 *)
+    let t2 = it_sqr1 50 t2 in  (* z_250_50 *)
+    let t1 =  Zp_25519.( * ) t1 t2 in        (* z_250_0 *)
+    let t1 = it_sqr1 4 t1 in   (* z_255_5 *) 
+    let t1 = sqr t1 in
+    let t1 =  Zp_25519.( * ) t0 t1 in
+        t1 axiomatized by invert2E.
 
 lemma eq_invert2 (z1: zp) :
-  invert2 z1 = invert1 z1.
+    invert2 z1 = invert1 z1.
 proof.
-  rewrite invert2E invert1E. smt(eq_it_sqr1).
+    rewrite invert2E invert1E. smt(eq_it_sqr1).
 qed.
 
 lemma eq_invert210p (z1: zp) :
-  invert2 z1 = ZModpRing.exp z1 (p-2).
+    invert2 z1 = ZModpRing.exp z1 (p-2).
 proof.
-rewrite eq_invert2 eq_invert1 eq_invert0p //.
+    rewrite eq_invert2 eq_invert1 eq_invert0p //.
 qed.
 
 (* now we define an alternative version of encodePoint *)
 op encodePoint1 (q: zp * zp) : W256.t =
-  let qi = invert2 q.`2 in
-  let q =  Zp_25519.( * ) q.`1 qi in
-      W256.of_int (asint q) axiomatized by encodePoint1E.
+    let qi = invert2 q.`2 in
+    let q =  Zp_25519.( * ) q.`1 qi in
+        W256.of_int (asint q) axiomatized by encodePoint1E.
 
 lemma eq_encodePoint1 (q: zp * zp) :
-  encodePoint1 q = encodePoint q.
+    encodePoint1 q = encodePoint q.
 proof.
-  rewrite encodePoint1E encodePointE. simplify. congr.
-  rewrite eq_invert210p //.
+    rewrite encodePoint1E encodePointE. simplify. congr.
+    rewrite eq_invert210p //.
 qed.
 
 (** step 6: scalarmult with updated montgomery_ladder3 **)
 
 op scalarmult_internal1(u: zp) (k:W256.t) : W256.t =
-   let r = montgomery_ladder3 u  k in
-   encodePoint1 (r.`1) axiomatized by scalarmult_internal1E.
+    let r = montgomery_ladder3 u  k in
+        encodePoint1 (r.`1) axiomatized by scalarmult_internal1E.
 
 (* lemma scalarmult = scalarmult1 *)
 lemma eq_scalarmult_internal1 (u:zp) (k:W256.t) :
-  k.[0] = false => scalarmult_internal1 u k = scalarmult_internal u k.
-  proof.
-  rewrite /scalarmult_internal1. simplify.
-  rewrite eq_encodePoint1 /scalarmult_internal.
-  simplify. move => H. 
-  congr.
-  have ml123 : montgomery_ladder u k = select_tuple_12 (montgomery_ladder3 u k).
-  apply eq_montgomery_ladder123. apply H.
-  rewrite ml123 /select_tuple_12 //.
+    k.[0] = false => scalarmult_internal1 u k = scalarmult_internal u k.
+proof.
+    rewrite /scalarmult_internal1. simplify.
+    rewrite eq_encodePoint1 /scalarmult_internal.
+    simplify. move => H. 
+    congr.
+    have ml123 : montgomery_ladder u k = select_tuple_12 (montgomery_ladder3 u k).
+        apply eq_montgomery_ladder123. apply H.
+    rewrite ml123 /select_tuple_12 //.
 qed.
 
 hint simplify scalarmult_internal1E.
 
 op scalarmult1 (k:W256.t) (u:W256.t) : W256.t =
-  let k = decodeScalar25519 k in
-  let u = decodeUCoordinate u in
-  scalarmult_internal1 u k axiomatized by scalarmult1E.
+    let k = decodeScalar25519 k in
+    let u = decodeUCoordinate u in
+    scalarmult_internal1 u k axiomatized by scalarmult1E.
  
 hint simplify scalarmult1E.
 
 op scalarmult_base1(k:W256.t) : W256.t =
-  scalarmult1 (k) (W256.of_int(9%Int)).
+    scalarmult1 (k) (W256.of_int(9%Int)).
 
 (* lemma scalarmult = scalarmult1 *)
 lemma eq_scalarmult1 (k:W256.t) (u:W256.t) :
-  scalarmult1 k u = scalarmult k u.
+    scalarmult1 k u = scalarmult k u.
 proof.
-  simplify.
-  pose du := decodeUCoordinate u.
-  pose dk := decodeScalar25519 k.
-  rewrite eq_encodePoint1 /scalarmult_internal. simplify.
-  congr.
-  have kb0f  : (dk).[0] = false. (* k bit 0 false *)
-    rewrite /dk /decodeScalar25519 //.
-  have ml123 : montgomery_ladder du dk = select_tuple_12 (montgomery_ladder3 du dk).
-    move : kb0f. apply eq_montgomery_ladder123.
-  rewrite ml123 /select_tuple_12 //.
+    simplify.
+    pose du := decodeUCoordinate u.
+    pose dk := decodeScalar25519 k.
+    rewrite eq_encodePoint1 /scalarmult_internal. simplify.
+    congr.
+    have kb0f  : (dk).[0] = false. (* k bit 0 false *)
+        rewrite /dk /decodeScalar25519 //.
+    have ml123 : montgomery_ladder du dk = select_tuple_12 (montgomery_ladder3 du dk).
+        move : kb0f. apply eq_montgomery_ladder123.
+    rewrite ml123 /select_tuple_12 //.
 qed.
 
 lemma eq_scalarmult_base1 (k:W256.t) :
     scalarmult_base1 k = scalarmult_base k.
 proof.
-  apply eq_scalarmult1.
+    apply eq_scalarmult1.
 qed.
 
 
