src/Curve25519_Hop4.ec
@@ -15,62 +15,64 @@ import Curve25519_Spec Curve25519_auto Curve25519_Hop1 Curve25519_Hop2 Curve2551
 
 equiv eq_h4_init_points :
     MHop2.init_points ~ M.__init_points4 : 
-init{1} = inzpRep4 initr{2}
-==> 
-res{1}.`1 = inzpRep4 res{2}.`1 /\
-res{1}.`2 = inzpRep4 res{2}.`2 /\
-res{1}.`3 = inzpRep4 res{2}.`3 /\
-res{1}.`4 = inzpRep4 res{2}.`4.
+        init{1} = inzpRep4 initr{2}
+        ==> 
+        res{1}.`1 = inzpRep4 res{2}.`1 /\
+        res{1}.`2 = inzpRep4 res{2}.`2 /\
+        res{1}.`3 = inzpRep4 res{2}.`3 /\
+        res{1}.`4 = inzpRep4 res{2}.`4.
 proof.
-proc. 
-wp. unroll for{2} ^while. wp. skip. move => &1 &2 H H0 H1 H2 H3 H4 H5 H6.
-split; auto => />. rewrite /H4 /H0 /H2 /H3 /Zp_25519.one /set0_64_ /inzpRep4 => />.
-rewrite /valRep4 /to_list /mkseq -iotaredE => />.
-split; auto => />. rewrite /H5  /H0 /H3 /H2 /Zp_25519.zero /set0_64_ /inzpRep4 => />.
-rewrite /valRep4 /to_list /mkseq -iotaredE  => />.
-rewrite /H6  /H0 /H3 /H2 /Zp_25519.zero /set0_64_ /inzpRep4 // /valRep4 /to_list /mkseq -iotaredE  => />.
+    proc. 
+    wp. unroll for{2} ^while. wp. skip. move => &1 &2 H H0 H1 H2 H3 H4 H5 H6.
+    split; auto => />. rewrite /H4 /H0 /H2 /H3 /Zp_25519.one /set0_64_ /inzpRep4 => />.
+        rewrite /valRep4 /to_list /mkseq -iotaredE => />.
+    split; auto => />. rewrite /H5  /H0 /H3 /H2 /Zp_25519.zero /set0_64_ /inzpRep4 => />.
+        rewrite /valRep4 /to_list /mkseq -iotaredE  => />.
+    rewrite /H6  /H0 /H3 /H2 /Zp_25519.zero /set0_64_ /inzpRep4 // /valRep4 /to_list /mkseq -iotaredE  => />.
 qed. 
 
 equiv eq_h4_decode_u_coordinate_base :
-  MHop2.decode_u_coordinate_base ~ M.__decode_u_coordinate_base4:
-  true ==> res{1} = inzpRep4 res{2}.
+    MHop2.decode_u_coordinate_base ~ M.__decode_u_coordinate_base4:
+        true 
+        ==> 
+        res{1} = inzpRep4 res{2}.
 proof.
-proc. wp. skip. move => &1 &2 H.
-rewrite /inzpRep4. congr. rewrite /valRep4 /to_list /mkseq -iotaredE => />.
+    proc. wp. skip. move => &1 &2 H.
+    rewrite /inzpRep4. congr. rewrite /valRep4 /to_list /mkseq -iotaredE => />.
 qed.
 
 
 (** step 4 : cswap **)
 equiv eq_h4_cswap :
-  MHop2.cswap ~ M.__cswap4:
-  x2{1}         = inzpRep4 x2{2}  /\
-  z2{1}         = inzpRep4 z2r{2} /\
-  x3{1}         = inzpRep4 x3{2}  /\
-  z3{1}         = inzpRep4 z3{2}  /\
-  b2i toswap{1} = to_uint toswap{2}
-  ==>
-  res{1}.`1     = inzpRep4 res{2}.`1  /\
-  res{1}.`2     = inzpRep4 res{2}.`2  /\
-  res{1}.`3     = inzpRep4 res{2}.`3  /\
-  res{1}.`4     = inzpRep4 res{2}.`4.
+    MHop2.cswap ~ M.__cswap4:
+        x2{1}         = inzpRep4 x2{2}      /\
+        z2{1}         = inzpRep4 z2r{2}     /\
+        x3{1}         = inzpRep4 x3{2}      /\
+        z3{1}         = inzpRep4 z3{2}      /\
+        b2i toswap{1} = to_uint toswap{2}
+        ==>
+        res{1}.`1     = inzpRep4 res{2}.`1  /\
+        res{1}.`2     = inzpRep4 res{2}.`2  /\
+        res{1}.`3     = inzpRep4 res{2}.`3  /\
+        res{1}.`4     = inzpRep4 res{2}.`4.
 proof.
-proc.
-do 4! unroll for{2} ^while.
-case: (toswap{1}).
-  rcondt {1} 1 => //. wp => /=. skip.
-    move => &1 &2 [#] 4!->> ??.
-    have mask_set :  (set0_64.`6 - toswap{2}) = W64.onew. rewrite /set0_64_ /=. smt(@W64).
-    rewrite !mask_set /=.
-    have lxor1 : forall (x1 x2:W64.t),  x1 `^` (x2 `^` x1) = x2.
-      move=> *. rewrite xorwC -xorwA xorwK xorw0 //.
-    have lxor2 : forall (x1 x2:W64.t),  x1 `^` (x1 `^` x2) = x2.
-      move=> *. rewrite xorwA xorwK xor0w //. 
-  rewrite !lxor1 !lxor2.
-      split. congr. apply Array4.ext_eq. smt(@Array4).
-      split. congr. apply Array4.ext_eq. smt(@Array4).
-      split. congr. apply Array4.ext_eq. smt(@Array4).
-             congr. apply Array4.ext_eq. smt(@Array4).
-  rcondf {1} 1 => //. wp => /=; skip.
+    proc.
+    do 4! unroll for{2} ^while.
+    case: (toswap{1}).
+        rcondt {1} 1 => //. wp => /=. skip.
+        move => &1 &2 [#] 4!->> ??.
+        have mask_set :  (set0_64.`6 - toswap{2}) = W64.onew. rewrite /set0_64_ /=. smt(@W64).
+        rewrite !mask_set /=.
+        have lxor1 : forall (x1 x2:W64.t),  x1 `^` (x2 `^` x1) = x2.
+            move=> *. rewrite xorwC -xorwA xorwK xorw0 //.
+        have lxor2 : forall (x1 x2:W64.t),  x1 `^` (x1 `^` x2) = x2.
+            move=> *. rewrite xorwA xorwK xor0w //. 
+        rewrite !lxor1 !lxor2.
+        split. congr. apply Array4.ext_eq. smt(@Array4).
+        split. congr. apply Array4.ext_eq. smt(@Array4).
+        split. congr. apply Array4.ext_eq. smt(@Array4).
+        congr. apply Array4.ext_eq. smt(@Array4).
+    rcondf {1} 1 => //. wp => /=; skip.
     move => &1 &2 [#] 4!->> ??.
     have mask_not_set :  (set0_64.`6 - toswap{2}) = W64.zero. smt(@W64).
     rewrite !mask_not_set !andw0 !xorw0.
@@ -79,57 +81,57 @@ qed.
 
 (** step 5 : add_and_double **)
 equiv eq_h4_add_and_double :
-  MHop2.add_and_double ~ M.__add_and_double4:
-  init{1} = inzpRep4 init{2} /\
-  x2{1}   = inzpRep4 x2{2}   /\
-  z2{1}   = inzpRep4 z2r{2}  /\
-  x3{1}   = inzpRep4 x3{2}   /\
-  z3{1}   = inzpRep4 z3{2}
-  ==>
-  res{1}.`1 = inzpRep4 res{2}.`1 /\
-  res{1}.`2 = inzpRep4 res{2}.`2 /\
-  res{1}.`3 = inzpRep4 res{2}.`3 /\
-  res{1}.`4 = inzpRep4 res{2}.`4.
+    MHop2.add_and_double ~ M.__add_and_double4:
+        init{1} = inzpRep4 init{2}     /\
+        x2{1}   = inzpRep4 x2{2}       /\
+        z2{1}   = inzpRep4 z2r{2}      /\
+        x3{1}   = inzpRep4 x3{2}       /\
+        z3{1}   = inzpRep4 z3{2}
+        ==>
+        res{1}.`1 = inzpRep4 res{2}.`1 /\
+        res{1}.`2 = inzpRep4 res{2}.`2 /\
+        res{1}.`3 = inzpRep4 res{2}.`3 /\
+        res{1}.`4 = inzpRep4 res{2}.`4.
 proof.
-proc => /=.
-  call eq_h4_mul_rss.
-  call eq_h4_mul_sss.
-  call eq_h4_add_sss.
-  call eq_h4_sqr_ss_.
-  call eq_h4_mul_a24_ss.
-  call eq_h4_sqr_ss_.
-  call eq_h4_sub_sss.
-  call eq_h4_mul_sss.
-  call eq_h4_sub_sss.
-  call eq_h4_add_sss.
-  call eq_h4_sqr_ss_.
-  call eq_h4_sqr_ss_.
-  call eq_h4_mul_sss.
-  call eq_h4_mul_sss.
-  call eq_h4_add_sss.
-  call eq_h4_sub_sss.
-  call eq_h4_add_ssr.
-  call eq_h4_sub_ssr.
-  wp. done.
+    proc => /=.
+    call eq_h4_mul_rss.
+    call eq_h4_mul_sss.
+    call eq_h4_add_sss.
+    call eq_h4_sqr_ss_.
+    call eq_h4_mul_a24_ss.
+    call eq_h4_sqr_ss_.
+    call eq_h4_sub_sss.
+    call eq_h4_mul_sss.
+    call eq_h4_sub_sss.
+    call eq_h4_add_sss.
+    call eq_h4_sqr_ss_.
+    call eq_h4_sqr_ss_.
+    call eq_h4_mul_sss.
+    call eq_h4_mul_sss.
+    call eq_h4_add_sss.
+    call eq_h4_sub_sss.
+    call eq_h4_add_ssr.
+    call eq_h4_sub_ssr.
+    wp. done.
 qed.
 
 (** step 6 : montgomery_ladder_step **)
 equiv eq_h4_montgomery_ladder_step :
- MHop2.montgomery_ladder_step ~ M.__montgomery_ladder_step4:
-   inzp (to_uint k'{1}) =   inzpRep32 k{2} /\
-   init'{1} = inzpRep4 init{2} /\
-   x2{1} = inzpRep4 x2{2} /\
-   z2{1} = inzpRep4 z2r{2} /\
-   x3{1} = inzpRep4 x3{2} /\
-   z3{1} = inzpRep4 z3{2} /\ 
-   b2i swapped{1} = to_uint swapped{2} /\
-   ctr'{1} = to_uint ctr{2}
-   ==>
-   res{1}.`1 = inzpRep4 res{2}.`1 /\
-   res{1}.`2 = inzpRep4 res{2}.`2 /\
-   res{1}.`3 = inzpRep4 res{2}.`3 /\
-   res{1}.`4 = inzpRep4 res{2}.`4 /\
-   b2i res{1}.`5 = to_uint res{2}.`5.
+    MHop2.montgomery_ladder_step ~ M.__montgomery_ladder_step4:
+        inzp (to_uint k'{1}) =   inzpRep32 k{2} /\
+        init'{1} = inzpRep4 init{2}             /\
+        x2{1} = inzpRep4 x2{2}                  /\
+        z2{1} = inzpRep4 z2r{2}                 /\
+        x3{1} = inzpRep4 x3{2}                  /\
+        z3{1} = inzpRep4 z3{2}                  /\ 
+        b2i swapped{1} = to_uint swapped{2}     /\
+        ctr'{1} = to_uint ctr{2}
+        ==>
+        res{1}.`1 = inzpRep4 res{2}.`1          /\
+        res{1}.`2 = inzpRep4 res{2}.`2          /\
+        res{1}.`3 = inzpRep4 res{2}.`3          /\
+        res{1}.`4 = inzpRep4 res{2}.`4          /\
+        b2i res{1}.`5 = to_uint res{2}.`5.
 proof.
     proc => /=. 
     call eq_h4_add_and_double. wp.
@@ -147,17 +149,17 @@ qed.
 
 (** step 7 : montgomery_ladder **)
 equiv eq_h4_montgomery_ladder :
-  MHop2.montgomery_ladder ~ M.__montgomery_ladder4 :
-   init'{1} = inzpRep4 u{2} /\
-    inzp (W256.to_uint k'{1}) =  inzpRep32 k{2}
-   ==>
-   res{1}.`1 = inzpRep4 res{2}.`1 /\
-   res{1}.`2 =inzpRep4  res{2}.`2.
+    MHop2.montgomery_ladder ~ M.__montgomery_ladder4 :
+        init'{1} = inzpRep4 u{2}                     /\
+        inzp (W256.to_uint k'{1}) =  inzpRep32 k{2}
+        ==>
+        res{1}.`1 = inzpRep4 res{2}.`1               /\
+        res{1}.`2 =inzpRep4  res{2}.`2.
 proof.
     proc. wp. sp. 
     unroll {1} 4. 
     rcondt {1} 4. progress. inline MHop2.init_points.
-    wp. sp. skip. progress.
+        wp. sp. skip. progress.
     while(
           inzp (to_uint k'{1}) = inzpRep32 k{2}             /\ 
           ctr{1} = to_uint ctr{2}                          /\ 
@@ -168,169 +170,185 @@ proof.
           z2{1} = inzpRep4 z2r{2}                          /\
           z3{1} = inzpRep4 z3{2}                           /\
           b2i swapped{1} = to_uint swapped{2}).
-    wp. sp. call eq_h4_montgomery_ladder_step. skip. progress.
-    rewrite to_uintB. rewrite uleE to_uint1 => />. smt(). rewrite to_uint1 => />.
-    rewrite ultE to_uintB. rewrite uleE to_uint1. smt().
-    rewrite to_uint1 to_uint0. trivial. smt(@W64).  
+        wp. sp. call eq_h4_montgomery_ladder_step. skip. progress.
+                rewrite to_uintB. rewrite uleE to_uint1 => />. smt(). rewrite to_uint1 => />.
+            rewrite ultE to_uintB. rewrite uleE to_uint1. smt().
+            rewrite to_uint1 to_uint0. trivial. smt(@W64).  
     call eq_h4_montgomery_ladder_step. wp. call eq_h4_init_points. skip. done.
 qed.
 
- (** step 8 : iterated square, may be error in variable names, ened to chec  **)
 (** step 8 : iterated square **)
 equiv eq_h4_it_sqr :
- MHop2.it_sqr ~ M._it_sqr4_p:
-   f{1}            =    inzpRep4 x{2} /\
-   i{1}            =    to_uint i{2}  /\
-   2               <=   to_uint i{2}  /\
-   i{1}            <=   W32.modulus   /\
-   0              <=   i{1}   ==>
-   res{1} = inzpRep4 res{2}.
+    MHop2.it_sqr ~ M._it_sqr4_p:
+        f{1}            =    inzpRep4 x{2} /\
+        i{1}            =    to_uint i{2}  /\
+        2               <=   to_uint i{2}  /\
+        i{1}            <=   W32.modulus   /\
+        0               <=   i{1}   
+        ==>
+        res{1} = inzpRep4 res{2}.
 proof.
-proc. simplify. wp. sp.
-  while (h{1}            =    inzpRep4 x{2}            /\ 
+    proc. simplify. wp. sp.
+    while (h{1}            =    inzpRep4 x{2}            /\ 
          ii{1}            =    to_uint i{2}             /\
          ii{1}            <=   W32.modulus              /\
          0                <=   ii{1}                     
-).
-   wp. call eq_h4_sqr_p. conseq(_: _ ==> h{1} = inzpRep4 x{2}).
-   progress. rewrite /DEC_32 /rflags_of_aluop_nocf_w /ZF_of => /=.
-   smt(@W32). smt().  smt(@W32). 
-   rewrite /DEC_32 /rflags_of_aluop_nocf_w /ZF_of => /=. smt(@W32).
-   rewrite /DEC_32 /rflags_of_aluop_nocf_w /ZF_of => /=. smt(@W32).
-   skip. progress. wp. 
-   call eq_h4_sqr_p.  
-   skip. progress.
-   rewrite /DEC_32 /rflags_of_aluop_nocf_w /ZF_of => /=. smt(@W32). smt(). smt(@W32).
-   rewrite /DEC_32 /rflags_of_aluop_nocf_w /ZF_of => /=. smt(@W32). smt().
+    ).
+    wp. call eq_h4_sqr_p. conseq(_: _ ==> h{1} = inzpRep4 x{2}).
+    progress. rewrite /DEC_32 /rflags_of_aluop_nocf_w /ZF_of => /=.
+    smt(@W32). smt().  smt(@W32). 
+    rewrite /DEC_32 /rflags_of_aluop_nocf_w /ZF_of => /=. smt(@W32).
+    rewrite /DEC_32 /rflags_of_aluop_nocf_w /ZF_of => /=. smt(@W32).
+    skip. progress. wp. 
+    call eq_h4_sqr_p.  
+    skip. progress.
+    rewrite /DEC_32 /rflags_of_aluop_nocf_w /ZF_of => /=. smt(@W32). smt(). smt(@W32).
+    rewrite /DEC_32 /rflags_of_aluop_nocf_w /ZF_of => /=. smt(@W32). smt().
 qed.
 
 equiv eq_h4_it_sqr_s :
- MHop2.it_sqr ~ M._it_sqr4_s_:
-   f{1}            =    inzpRep4 x{2} /\
-   i{1}            =    to_uint i{2}  /\
-   2               <=   to_uint i{2}  /\
-   i{1}            <=   W32.modulus   /\
-    2              <=   i{1}   ==>
-   res{1} = inzpRep4 res{2}.
+    MHop2.it_sqr ~ M._it_sqr4_s_:
+        f{1}            =    inzpRep4 x{2} /\
+        i{1}            =    to_uint i{2}  /\
+        2               <=   to_uint i{2}  /\
+        i{1}            <=   W32.modulus   /\
+        2              <=   i{1}   ==>
+        res{1} = inzpRep4 res{2}.
 proof.
- proc. simplify. wp. sp.
-admit.
+    proc. simplify. wp. sp.
+    admit.
 qed.
 
 equiv eq_h4_it_sqr_ss :
- MHop2.it_sqr ~ M._it_sqr4_ss_:
-   f{1}            =    inzpRep4 x{2} /\
-   i{1}            =    W32.to_uint i{2}
-   ==>
-   res{1} = inzpRep4 res{2}.
+        MHop2.it_sqr ~ M._it_sqr4_ss_:
+    f{1}            =    inzpRep4 x{2} /\
+    i{1}            =    W32.to_uint i{2}
+    ==>
+    res{1} = inzpRep4 res{2}.
 proof.
- proc. wp. sp. inline M._it_sqr4_p. sp. wp. admit.
+    proc. wp. sp. inline M._it_sqr4_p. sp. wp. admit.
 qed.
 
 (** step 9 : invert **)
 equiv eq_h4_invert :
-  MHop2.invert ~ M.__invert4 : 
-     fs{1} = inzpRep4 fs{2}
-  ==> res{1} = inzpRep4 res{2}.
+    MHop2.invert ~ M.__invert4 : 
+        fs{1} = inzpRep4 fs{2}
+        ==> 
+        res{1} = inzpRep4 res{2}.
 proof.
-  proc.
-  sp.
-  call eq_h4_mul_ss.
-  call eq_h4_sqr_s_.
-  call (eq_h4_it_sqr_s). wp.
-  call eq_h4_mul_ss.
-  call eq_h4_it_sqr_s. wp.
-  call eq_h4_mul_ss.
-  call eq_h4_it_sqr_ss. wp.
-  call eq_h4_mul_ss.
-  call eq_h4_it_sqr_ss. wp.
-  call eq_h4_mul_ss.
-  call eq_h4_it_sqr_s. wp.
-  call eq_h4_mul_ss.
-  call eq_h4_it_sqr_ss. wp.
-  call eq_h4_mul_ss.
-  call eq_h4_it_sqr_ss. wp.
-  call eq_h4_mul_ss.
-  call eq_h4_it_sqr_s. wp.
-  call eq_h4_sqr_ss.
-  call eq_h4_mul_ss.
-  call eq_h4_sqr_ss.
-  call eq_h4_mul_ss.
-  call eq_h4_mul_ss.
-  call eq_h4_sqr_s_.
-  call eq_h4_sqr_ss.
-  call eq_h4_sqr_ss. wp. 
-  skip. done.
+    proc.
+    sp.
+    call eq_h4_mul_ss.
+    call eq_h4_sqr_s_.
+    call (eq_h4_it_sqr_s). wp.
+    call eq_h4_mul_ss.
+    call eq_h4_it_sqr_s. wp.
+    call eq_h4_mul_ss.
+    call eq_h4_it_sqr_ss. wp.
+    call eq_h4_mul_ss.
+    call eq_h4_it_sqr_ss. wp.
+    call eq_h4_mul_ss.
+    call eq_h4_it_sqr_s. wp.
+    call eq_h4_mul_ss.
+    call eq_h4_it_sqr_ss. wp.
+    call eq_h4_mul_ss.
+    call eq_h4_it_sqr_ss. wp.
+    call eq_h4_mul_ss.
+    call eq_h4_it_sqr_s. wp.
+    call eq_h4_sqr_ss.
+    call eq_h4_mul_ss.
+    call eq_h4_sqr_ss.
+    call eq_h4_mul_ss.
+    call eq_h4_mul_ss.
+    call eq_h4_sqr_s_.
+    call eq_h4_sqr_ss.
+    call eq_h4_sqr_ss. wp. 
+    skip. done.
 qed.
-
 
 
 (** step 11 : scalarmult **)
 
 equiv eq_h4_scalarmult_internal :
-  MHop2.scalarmult_internal ~ M.__curve25519_internal_ref4:
-  inzp(W256.to_uint k'{1}) = inzpRep32 k{2} /\  u''{1} = inzpRep4 u{2}
-  ==>
-  inzp(W256.to_uint res{1}) = inzpRep4 res{2}. 
+    MHop2.scalarmult_internal ~ M.__curve25519_internal_ref4:
+        inzp(W256.to_uint k'{1}) = inzpRep32 k{2} /\  
+        u''{1} = inzpRep4 u{2}
+        ==>
+        inzp(W256.to_uint res{1}) = inzpRep4 res{2}. 
 proof.
-proc.
-call eq_h4_encode_point.
-call eq_h4_montgomery_ladder. wp. skip.
-done.
+    proc.
+    call eq_h4_encode_point.
+    call eq_h4_montgomery_ladder. wp. skip.
+    done.
 qed.
 
 equiv eq_h4_scalarmult :
-  MHop2.scalarmult ~ M._curve25519_ref4:
-  inzp(W256.to_uint k'{1}) = inzpRep4 _k{2} /\  inzp (to_uint u'{1}) = inzpRep4 _u{2}
-  ==>
-  inzp(W256.to_uint res{1}) = inzpRep4 res{2}. 
+    MHop2.scalarmult ~ M._curve25519_ref4:
+        inzp(W256.to_uint k'{1}) = inzpRep4 _k{2} /\  
+        inzp (to_uint u'{1}) = inzpRep4 _u{2}
+        ==>
+        inzp(W256.to_uint res{1}) = inzpRep4 res{2}. 
 proof.
-proc.
-call eq_h4_scalarmult_internal => />.
-call eq_h4_decode_u_coordinate => />.
-call eq_h4_decode_scalar_25519.
-wp. skip. progress.
+    proc.
+    call eq_h4_scalarmult_internal => />.
+    call eq_h4_decode_u_coordinate => />.
+    call eq_h4_decode_scalar_25519.
+    wp. skip. progress.
 qed.
 
 
 equiv eq_h4_scalarmult_ptr : (* how to get address *)
-  MHop2.scalarmult ~ M.__curve25519_ref4_ptr:
-  true ==> true.
+    MHop2.scalarmult ~ M.__curve25519_ref4_ptr:
+        true
+        ==> 
+        true.
 proof.
-admit.
+    proc *.
+    inline M.__curve25519_ref4_ptr. 
+    sp. wp. inline M.__load4 M.__store4. do 3! unroll for{2} ^while.
+    sp. wp. 
+    call eq_h4_scalarmult. skip. progress.
+    admit. admit.
 qed.
 
 
 equiv eq_h4_scalarmult_base :
-  MHop2.scalarmult_base ~ M._curve25519_ref4_base:
-  inzp(W256.to_uint k'{1}) = inzpRep4 _k{2} ==>  inzp(W256.to_uint res{1}) = inzpRep4 res{2}. 
+    MHop2.scalarmult_base ~ M._curve25519_ref4_base:
+        inzp(W256.to_uint k'{1}) = inzpRep4 _k{2} 
+        ==>  
+        inzp(W256.to_uint res{1}) = inzpRep4 res{2}. 
 proof.
-proc.
-call eq_h4_scalarmult_internal => />.
-call eq_h4_decode_u_coordinate_base => />.
-call eq_h4_decode_scalar_25519.
-wp. skip. progress.
+    proc.
+    call eq_h4_scalarmult_internal => />.
+    call eq_h4_decode_u_coordinate_base => />.
+    call eq_h4_decode_scalar_25519.
+    wp. skip. progress.
 qed.
 
 equiv eq_h4_scalarmult_base_ptr :
-  MHop2.scalarmult_base ~ M.__curve25519_ref4_base_ptr:
-  true ==> true.
+    MHop2.scalarmult_base ~ M.__curve25519_ref4_base_ptr:
+        true 
+        ==> 
+        true.
 proof.
-admit.
+    admit.
 qed.
 
 
 equiv eq_h4_scalarmult_jade :
-  MHop2.scalarmult ~ M.jade_scalarmult_curve25519_amd64_ref4:
-  true
-  ==>
-  true.
-admit.
+    MHop2.scalarmult ~ M.jade_scalarmult_curve25519_amd64_ref4:
+        true
+        ==>
+        true.
+proof.
+    admit.
 qed.
 
 equiv eq_h4_scalarmult_jade_base :
-  MHop2.scalarmult_base ~ M.jade_scalarmult_curve25519_amd64_ref4_base:
-  true ==> true.
+    MHop2.scalarmult_base ~ M.jade_scalarmult_curve25519_amd64_ref4_base:
+        true 
+        ==> 
+        true.
 proof.
-admit.
+    admit.
 qed.
